examples/Baby.v
@@ -1,0 +1,64 @@
+Require Import Bedrock.
+
+
+(** The simplest function *)
+
+Definition diverger := bmodule "diverger" {{
+  bfunction "diverger" [st ~> [|True|] ] {
+    Diverge
+  }
+}}.
+
+Eval compute in compile diverger.
+
+Theorem divergerOk : moduleOk diverger.
+  structured.
+Qed.
+
+Print Assumptions divergerOk.
+
+
+(** Immediate return *)
+
+Definition immedS : assert := st ~> st#Rp @@ (st' ~> [| True |]).
+
+Definition immed := bmodule "immed" {{
+  bfunction "immed" [immedS] {
+    Goto Rp
+  }
+}}.
+
+Eval compute in compile immed.
+
+Theorem immedOk : moduleOk immed.
+  structured; ho.
+Qed.
+
+Print Assumptions immedOk.
+
+Definition immedTest := bimport [[ "immed"!"immed" @ [immedS] ]]
+  bmodule "main" {{
+    bfunction "main" [st ~> [| True |] ] {
+      Call "immed"!"immed"
+      [st ~> [| True |] ];;
+      Diverge
+    }
+  }}.
+
+Eval compute in compile immedTest.
+
+Theorem immedTestOk : moduleOk immedTest.
+  structured; ho.
+Qed.
+
+Print Assumptions immedTestOk.
+
+Definition immedProg := link immed immedTest.
+
+Eval compute in compile immedProg.
+
+Theorem immedProgOk : moduleOk immedProg.
+  link immedOk immedTestOk.
+Qed.
+
+Print Assumptions immedProgOk.
