src/Bedrock.v
@@ -1,0 +1,5 @@
+Require Export String List.
+
+Require Export Nomega Word IL LabelMap PropX PropXTac XCAP Structured StructuredModule Programming.
+
+Open Scope string_scope.
