src/Programming.v
@@ -1,0 +1,178 @@
+(* Final syntax for structured programming *)
+
+Require Import Bool String.
+
+Require Import PropX PropXTac IL LabelMap XCAP Structured StructuredModule.
+
+Set Implicit Arguments.
+
+
+
+(** * The type of context-independent structured program chunks *)
+
+Inductive chunk :=
+| StraightLine : list instr -> chunk
+| Structured : list instr -> (forall im mn, importsGlobal im -> cmd im mn) -> chunk.
+
+Definition toCmd (ch : chunk) im mn (H : importsGlobal im) : cmd im mn :=
+  match ch with
+    | StraightLine is => Straightline_ im mn is
+    | Structured nil c => c im mn H
+    | Structured is c => Seq_ H (Straightline_ im mn is) (c im mn H)
+  end.
+
+Definition Seq (ch1 ch2 : chunk) : chunk :=
+  match ch1, ch2 with
+    | StraightLine is1, StraightLine is2 => StraightLine (is1 ++ is2)
+    | StraightLine is1, Structured is2 c => Structured (is1 ++ is2) c
+    | Structured is1 c1, _ => Structured is1 (fun im mn H => Seq_ H (c1 im mn H) (toCmd ch2 mn H))
+  end.
+
+Definition Instr (i : instr) : chunk :=
+  StraightLine (i :: nil).
+
+Definition Diverge : chunk :=
+  Structured nil (fun im mn _ => Diverge_ im mn).
+
+Definition Fail : chunk :=
+  Structured nil (fun im mn _ => Fail_ im mn).
+
+Definition Skip : chunk :=
+  Structured nil (fun im mn _ => Skip_ im mn).
+
+Definition Use_ (lemma : settings -> state -> Prop) (pf : forall stn st, lemma stn st) : chunk :=
+  Structured nil (fun im mn _ => Use_ im mn lemma pf).
+
+Record condition := {
+  COperand1 : rvalue;
+  CTest : test;
+  COperand2 : rvalue
+}.
+
+Definition If_ (c : condition) (Then Else : chunk) : chunk :=
+  Structured nil (fun im mn H => If_ H (COperand1 c) (CTest c) (COperand2 c) (toCmd Then mn H) (toCmd Else mn H)).
+
+Definition While_ (inv : assert) (c : condition) (Body : chunk) : chunk :=
+  Structured nil (fun im mn H => While_ H inv (COperand1 c) (CTest c) (COperand2 c) (toCmd Body mn H)).
+
+Definition Goto (rv : rvalue) : chunk :=
+  Structured nil (fun im mn H => match rv with
+                                   | RvLabel f => Goto_ H mn f
+                                   | _ => IGoto im mn rv
+                                 end).
+
+Definition Call_ (f : label) (afterCall : assert) : chunk :=
+  Structured nil (fun im mn H => Call_ H mn f afterCall).
+
+
+(** * Modules *)
+
+Definition bmodule_ (im : list import) (mn : string)
+  (fs : list (string * assert * chunk)) : module :=
+  bmodule_ im (List.map (fun p => let '(f, pre, ch) := p in (f, pre, fun im' H => toCmd ch mn H)) fs).
+
+Definition compile (m : module) : list (label * block) := List.map (fun x => let '(k, (_, b)) := x in (k, b)) (LabelMap.elements (XCAP.Blocks m)).
+
+
+(** * Notations *)
+
+(** ** Expressions *)
+
+Notation "$[ v ]" := (LvMem v) (at level 0, n at level 0) : SP_scope.
+Notation "$[ r + w ]" := (LvMem (Indir r w)) (at level 0, r at level 0, w at level 0) : SP_scope.
+
+Definition labl (mod func : string) : label := (mod, Global func).
+
+Infix "!" := labl (at level 0, only parsing) : SP_scope.
+
+Delimit Scope SP_scope with SP.
+
+
+(** ** Instructions *)
+
+Inductive rhs :=
+| Rvalue : rvalue -> rhs
+| Bop : rvalue -> binop -> rvalue -> rhs.
+
+Coercion Rvalue : rvalue >-> rhs.
+
+Notation "x + y" := (Bop x Plus y) : SP_scope.
+Notation "x - y" := (Bop x Minus y) : SP_scope.
+Notation "x * y" := (Bop x Times y) : SP_scope.
+
+Notation "x = y" := {| COperand1 := x; CTest := Eq; COperand2 := y |} : SP_scope.
+Notation "x < y" := {| COperand1 := x; CTest := Lt; COperand2 := y |} : SP_scope.
+
+Definition Assign' (lv : lvalue) (rh : rhs) :=
+  Instr (match rh with
+           | Rvalue rv => Assign lv rv
+           | Bop rv1 bo rv2 => Binop lv rv1 bo rv2
+         end).
+
+Infix "<-" := Assign' (no associativity, at level 90) : SP_scope.
+
+
+(** ** Commands *)
+
+Infix ";;" := Seq (right associativity, at level 95) : SP_scope.
+
+Notation "'Use' [ pf ]" := (Use_ _ (fun _ _ => pf%nat)) (no associativity, at level 95) : SP_scope.
+Notation "'Use' st [ pf ]" := (Use_ _ (fun _ st => pf%nat)) (no associativity, at level 95) : SP_scope.
+
+Notation "'If' c { b1 } 'else' { b2 }" := (If_ c b1 b2)
+  (no associativity, at level 95, c at level 0) : SP_scope.
+
+Notation "[ p ] 'While' c { b }" := (While_ p c b)
+  (no associativity, at level 95, c at level 0) : SP_scope.
+
+Notation "'Call' f [ p ]" := (Call_ f p)
+  (no associativity, at level 95) : SP_scope.
+
+
+(** ** Modules *)
+
+Notation "'bfunction' name [ p ] { b }" := (name, p, b%SP)
+  (no associativity, at level 95, only parsing) : SPfuncs_scope.
+Delimit Scope SPfuncs_scope with SPfuncs.
+
+Notation "{{ x 'with' .. 'with' y }}" := (cons x .. (cons y nil) ..) (only parsing) : SPfuncs_scope.
+Delimit Scope SPfuncs_scope with SPfuncs.
+
+Notation "'bmodule' name fs" := (bmodule_ nil name fs%SPfuncs) (no associativity, at level 95, name at level 0, only parsing).
+
+Notation "x ! y" := (x, y) (only parsing) : SPimps_scope.
+Notation "name @ [ p ]" := (let (x, y) := name in (x, y, p)) (at level 0, only parsing) : SPimps_scope.
+Notation "[[ x , .. , y ]]" := (cons x .. (cons y nil) ..) (only parsing) : SPimps_scope.
+
+Delimit Scope SPimps_scope with SPimps.
+
+Notation "'bimport' is 'bmodule' name fs" := (bmodule_ is%SPimps name fs%SPfuncs) (no associativity, at level 95, name at level 0, only parsing).
+
+
+(** ** Specs *)
+
+Notation "st ~> p" := (fun x : settings * state => let st := snd x in p%PropX%nat) (at level 100, only parsing).
+
+Infix "#" := Regs (no associativity, at level 0).
+Notation "st .[ a ]" := (Mem st a) (no associativity, at level 0).
+
+
+
+(** * Tactics *)
+
+Ltac structured := apply bmoduleOk; [ exact (refl_equal false) | exact I |
+  simpl; repeat (apply List.Forall_nil || apply List.Forall_cons); (simpl; propxFo) ].
+
+Ltac link t1 t2 := apply linkOk; [ apply t1 | apply t2
+  | exact (refl_equal false) | repeat split | repeat split | exact I ].
+
+Ltac ho := autorewrite with IL in *;
+  repeat match goal with
+           | [ |- ex _ ] => eexists
+           | [ |- _ /\ _ ] => split
+         end; eauto; cbv zeta; simpl; intros;
+  try match goal with
+        | [ H : ?X = Some _ |- ?X = Some (fun x => ?g x) ] => apply H
+        | [ H : forall x, interp _ (_ --> ?p x) |- interp _ (?p _) ] => apply (Imply_sound (H _)); propxFo
+        | [ |- interp _ _ ] => propxFo
+      end.
