Makefile
@@ -3,9 +3,11 @@
 all:
 	# BEWARE: This will probably take a long time!
 	$(MAKE) -C src
+	$(MAKE) -C examples
 
 clean:
 	$(MAKE) -C src clean
+	$(MAKE) -C examples clean
 
 dist:
 	hg archive -t tgz /tmp/bedrock.tgz
